Etst/Subtyping/Utils/ExprClearVars.lean
@@ -4,123 +4,123 @@ namespace Etst
 
 
 namespace Expr
-  def clearBvars_eq_bvar
+  def clearVars_eq_var
     {ub: Nat}
     (lt: x < ub)
   :
-    clearBvars (E := E) ub (.bvar x) = .bvar x
+    clearVars (E := E) ub (.var x) = .var x
   :=
     if_pos lt
   
-  def clearBvars_eq_none
+  def clearVars_eq_none
     {ub: Nat}
     (nlt: ¬ x < ub)
   :
-    clearBvars (E := E) ub (.bvar x) = none
+    clearVars (E := E) ub (.var x) = none
   :=
     if_neg nlt
   
-  def clearBvars_none_eq_none
+  def clearVars_none_eq_none
   :
-    clearBvars (E := E) n none = none
+    clearVars (E := E) n none = none
   :=
-    show (if 0 < n + 1 then bvar 0 else none).arbUn.compl = none from
+    show (if 0 < n + 1 then var 0 else none).arbUn.compl = none from
     if_pos (Nat.zero_lt_succ n) ▸ rfl
   
-  def clearBvars_idempotent (expr: Expr E):
-    (expr.clearBvars n).clearBvars n = expr.clearBvars n
+  def clearVars_idempotent (expr: Expr E):
+    (expr.clearVars n).clearVars n = expr.clearVars n
   :=
     match expr with
-    | .var _ _ => rfl
-    | .bvar x =>
+    | .const _ _ => rfl
+    | .var x =>
       if h: x < n then by
-        rw [clearBvars_eq_bvar h, clearBvars_eq_bvar h]
+        rw [clearVars_eq_var h, clearVars_eq_var h]
       else by
-        rw [clearBvars_eq_none h]
-        exact clearBvars_none_eq_none
+        rw [clearVars_eq_none h]
+        exact clearVars_none_eq_none
     | .null => rfl
     | .pair left rite =>
         congrArg₂ Expr.pair
-          left.clearBvars_idempotent
-          rite.clearBvars_idempotent
+          left.clearVars_idempotent
+          rite.clearVars_idempotent
     | .ir left rite =>
         congrArg₂ Expr.ir
-          left.clearBvars_idempotent
-          rite.clearBvars_idempotent
+          left.clearVars_idempotent
+          rite.clearVars_idempotent
     | .condFull body =>
-        congrArg Expr.condFull body.clearBvars_idempotent
+        congrArg Expr.condFull body.clearVars_idempotent
     | .compl body =>
-        congrArg Expr.compl body.clearBvars_idempotent
+        congrArg Expr.compl body.clearVars_idempotent
     | .arbIr body =>
-        congrArg Expr.arbIr (body.clearBvars_idempotent)
+        congrArg Expr.arbIr (body.clearVars_idempotent)
   
-  def clearBvars_isClean (expr: Expr E):
-    IsClean expr.clearBvars
+  def clearVars_isClean (expr: Expr E):
+    IsClean expr.clearVars
   :=
-    (clearBvars_idempotent expr).symm
+    (clearVars_idempotent expr).symm
   
 end Expr
 
 namespace SingleLaneExpr
   open Expr
   
-  def clearBvars_preserves_interp_bv
+  def clearVars_preserves_interp_bv
     (expr: SingleLaneExpr)
     (bv bvRest: List Pair)
     (b c: Valuation Pair)
   :
     Eq
       (expr.intp2 bv b c)
-      (intp2 (expr.clearBvars bv.length) (bv ++ bvRest) b c)
+      (intp2 (expr.clearVars bv.length) (bv ++ bvRest) b c)
   :=
     match expr with
-    | .var _ _ => rfl
-    | .bvar x =>
+    | .const _ _ => rfl
+    | .var x =>
       if h: x < bv.length then
         let ltExtra: x < (bv ++ bvRest).length := 
           h.trans_le (bv.length_le_append_rite bvRest)
-        let eq: clearBvars bv.length (bvar x) = bvar x :=
-          clearBvars_eq_bvar h
+        let eq: clearVars bv.length (var x) = var x :=
+          clearVars_eq_var h
         by
-        rw [intp2_bvar_eq_of_lt h, eq]
-        rw [intp2_bvar_eq_of_lt ltExtra]
+        rw [intp2_var_eq_of_lt h, eq]
+        rw [intp2_var_eq_of_lt ltExtra]
         rw [bv.getElem_append_left h]
       else
-        clearBvars_eq_none h ▸
-        SingleLaneExpr.intp2_bvar_eq_empty h ▸
+        clearVars_eq_none h ▸
+        SingleLaneExpr.intp2_var_eq_empty h ▸
         SingleLaneExpr.intp2_none_eq_empty.symm
     | .null => rfl
     | .pair left rite =>
       eq_intp2_pair_of_eq
-        (clearBvars_preserves_interp_bv left bv bvRest b c)
-        (clearBvars_preserves_interp_bv rite bv bvRest b c)
+        (clearVars_preserves_interp_bv left bv bvRest b c)
+        (clearVars_preserves_interp_bv rite bv bvRest b c)
     | .ir left rite =>
       eq_intp2_ir_of_eq
-        (clearBvars_preserves_interp_bv left bv bvRest b c)
-        (clearBvars_preserves_interp_bv rite bv bvRest b c)
+        (clearVars_preserves_interp_bv left bv bvRest b c)
+        (clearVars_preserves_interp_bv rite bv bvRest b c)
     | .condFull body =>
       eq_intp2_condFull_of_eq
-        (clearBvars_preserves_interp_bv body bv bvRest b c)
+        (clearVars_preserves_interp_bv body bv bvRest b c)
     | .compl body =>
-      let ih := clearBvars_preserves_interp_bv body bv bvRest c b
+      let ih := clearVars_preserves_interp_bv body bv bvRest c b
       eq_intp2_compl_of_eq ih
     | .arbIr body =>
       eq_intp2_arbIr_of_eq (fun dX =>
-        clearBvars_preserves_interp_bv (bvRest := bvRest) body (dX :: bv) b c)
+        clearVars_preserves_interp_bv (bvRest := bvRest) body (dX :: bv) b c)
   
-  def clearBvars_preserves_interp
+  def clearVars_preserves_interp
     (expr: SingleLaneExpr)
     (bv: List Pair)
     (b c: Valuation Pair)
   :
     Eq
       (expr.intp2 [] b c)
-      (intp2 expr.clearBvars bv b c)
+      (intp2 expr.clearVars bv b c)
   :=
-    clearBvars_preserves_interp_bv expr [] bv b c
+    clearVars_preserves_interp_bv expr [] bv b c
   
   namespace IsClean
-    def bvar_independent
+    def var_independent
       {expr: SingleLaneExpr}
       (isClean: expr.IsClean)
       (bv0 bv1: List Pair)
@@ -129,8 +129,8 @@ namespace SingleLaneExpr
       expr.intp2 bv0 b c = expr.intp2 bv1 b c
     :=
       isClean ▸
-      clearBvars_preserves_interp expr bv0 b c ▸
-      clearBvars_preserves_interp expr bv1 b c ▸
+      clearVars_preserves_interp expr bv0 b c ▸
+      clearVars_preserves_interp expr bv1 b c ▸
       rfl
 
     def changeBv
@@ -141,70 +141,70 @@ namespace SingleLaneExpr
     :
       expr.intp2 bv1 b c d
     :=
-      bvar_independent isClean bv0 bv1 b c ▸ dInExpr
+      var_independent isClean bv0 bv1 b c ▸ dInExpr
     
   end IsClean
 end SingleLaneExpr
 
 namespace BasicExpr
-  def clearBvars_lane_comm
+  def clearVars_lane_comm
     (expr: BasicExpr)
     (lane: Set3.Lane)
     (i: Nat := 0)
   :
     Eq
-      (Expr.clearBvars i (expr.toLane lane))
-      (BasicExpr.toLane (Expr.clearBvars i expr) lane)
+      (Expr.clearVars i (expr.toLane lane))
+      (BasicExpr.toLane (Expr.clearVars i expr) lane)
   :=
     match expr with
-    | .var x => rfl
-    | .bvar x => by
+    | .const x => rfl
+    | .var x => by
       show
         Eq
-          (Expr.clearBvars i (.bvar x))
-          (toLane (Expr.clearBvars i (.bvar x)) lane)
+          (Expr.clearVars i (.var x))
+          (toLane (Expr.clearVars i (.var x)) lane)
       if h: x < i then
-        rw [Expr.clearBvars_eq_bvar h, Expr.clearBvars_eq_bvar h]
+        rw [Expr.clearVars_eq_var h, Expr.clearVars_eq_var h]
         rfl
       else
-        rw [Expr.clearBvars_eq_none h, Expr.clearBvars_eq_none h]
+        rw [Expr.clearVars_eq_none h, Expr.clearVars_eq_none h]
         rfl
     | .null => rfl
     | .pair left rite =>
         congrArg₂
           SingleLaneExpr.pair
-          (clearBvars_lane_comm left lane i)
-          (clearBvars_lane_comm rite lane i)
+          (clearVars_lane_comm left lane i)
+          (clearVars_lane_comm rite lane i)
     | .ir left rite =>
         congrArg₂
           SingleLaneExpr.ir
-          (clearBvars_lane_comm left lane i)
-          (clearBvars_lane_comm rite lane i)
+          (clearVars_lane_comm left lane i)
+          (clearVars_lane_comm rite lane i)
     | .condFull body =>
         congrArg
           SingleLaneExpr.condFull
-          (clearBvars_lane_comm body lane i)
+          (clearVars_lane_comm body lane i)
     | .compl body =>
         congrArg
           SingleLaneExpr.compl
-          (clearBvars_lane_comm body lane.toggle i)
+          (clearVars_lane_comm body lane.toggle i)
     | .arbIr body =>
         congrArg
           SingleLaneExpr.arbIr
-          (clearBvars_lane_comm body lane (i + 1))
+          (clearVars_lane_comm body lane (i + 1))
   
-  def clearBvars_preserves_interp
+  def clearVars_preserves_interp
     (expr: BasicExpr)
     (bv: List Pair)
     (b c: Valuation Pair)
   :
-    expr.triIntp2 [] b c = triIntp2 expr.clearBvars bv b c
+    expr.triIntp2 [] b c = triIntp2 expr.clearVars bv b c
   :=
-    let eqBvDef := (expr.toLane .defLane).clearBvars_preserves_interp bv b c
-    let eqBvPos := (expr.toLane .posLane).clearBvars_preserves_interp bv b c
+    let eqBvDef := (expr.toLane .defLane).clearVars_preserves_interp bv b c
+    let eqBvPos := (expr.toLane .posLane).clearVars_preserves_interp bv b c
     Set3.eq
-      (eqBvDef.trans (clearBvars_lane_comm expr .defLane ▸ rfl))
-      (eqBvPos.trans (clearBvars_lane_comm expr .posLane ▸ rfl))
+      (eqBvDef.trans (clearVars_lane_comm expr .defLane ▸ rfl))
+      (eqBvPos.trans (clearVars_lane_comm expr .posLane ▸ rfl))
 end BasicExpr
 
 namespace DefList
@@ -217,8 +217,8 @@ namespace DefList
     (dl.getDef x).triIntp2 bv0 b c = (dl.getDef x).triIntp2 bv1 b c
   :=
     dl.isClean x ▸
-    BasicExpr.clearBvars_preserves_interp (dl.getDef x) bv0 b c ▸
-    BasicExpr.clearBvars_preserves_interp (dl.getDef x) bv1 b c ▸
+    BasicExpr.clearVars_preserves_interp (dl.getDef x) bv0 b c ▸
+    BasicExpr.clearVars_preserves_interp (dl.getDef x) bv1 b c ▸
     rfl
   
   def interp_eq_bv_def
@@ -251,7 +251,7 @@ namespace SingleLaneExpr
   def InWfm.of_in_def
     (inDef: InWfm bv dl ((dl.getDef x).toLane lane) d)
   :
-    InWfm [] dl (.var lane x) d
+    InWfm [] dl (.const lane x) d
   :=
     of_in_def_no_bv
       (match lane with
@@ -265,7 +265,7 @@ namespace SingleLaneExpr
         eqPos ▸ inDef)
   
   def InWfm.in_def
-    (inVar: InWfm [] dl (.var lane x) d)
+    (inVar: InWfm [] dl (.const lane x) d)
   :
     InWfm bv dl ((dl.getDef x).toLane lane) d
   :=
@@ -282,138 +282,138 @@ end SingleLaneExpr
 
 
 namespace Expr
-  def looseBvarUB
+  def freeVarUB
     (expr: Expr E)
     (depth: Nat := 0)
   :
     Nat
   :=
     match expr with
-    | .var _ _ => 0
-    | .bvar x => if x < depth then 0 else x + 1 - depth
+    | .const _ _ => 0
+    | .var x => if x < depth then 0 else x + 1 - depth
     | .null => 0
     | .pair left rite =>
-        Nat.max (left.looseBvarUB depth) (rite.looseBvarUB depth)
+        Nat.max (left.freeVarUB depth) (rite.freeVarUB depth)
     | .ir left rite =>
-        Nat.max (left.looseBvarUB depth) (rite.looseBvarUB depth)
-    | .condFull body => body.looseBvarUB depth
-    | .compl body => body.looseBvarUB depth
-    | .arbIr body => body.looseBvarUB depth
+        Nat.max (left.freeVarUB depth) (rite.freeVarUB depth)
+    | .condFull body => body.freeVarUB depth
+    | .compl body => body.freeVarUB depth
+    | .arbIr body => body.freeVarUB depth
   
-  def looseBvarUB_pair_lt_left
-    (h : (pair l r).looseBvarUB d < x)
+  def freeVarUB_pair_lt_left
+    (h : (pair l r).freeVarUB d < x)
   :
-    l.looseBvarUB d < x
+    l.freeVarUB d < x
   :=
     Nat.lt_of_le_of_lt (Nat.le_max_left _ _) h
   
-  def looseBvarUB_pair_lt_rite
-    (h : (pair l r).looseBvarUB d < x)
+  def freeVarUB_pair_lt_rite
+    (h : (pair l r).freeVarUB d < x)
   :
-    r.looseBvarUB d < x
+    r.freeVarUB d < x
   :=
     Nat.lt_of_le_of_lt (Nat.le_max_right _ _) h
   
-  def looseBvarUB_un_lt_left
-    (h : (un l r).looseBvarUB d < x)
+  def freeVarUB_un_lt_left
+    (h : (un l r).freeVarUB d < x)
   :
-    l.looseBvarUB d < x
+    l.freeVarUB d < x
   :=
     Nat.lt_of_le_of_lt (Nat.le_max_left _ _) h
   
-  def looseBvarUB_un_lt_rite
-    (h : (un l r).looseBvarUB d < x)
+  def freeVarUB_un_lt_rite
+    (h : (un l r).freeVarUB d < x)
   :
-    r.looseBvarUB d < x
+    r.freeVarUB d < x
   :=
     Nat.lt_of_le_of_lt (Nat.le_max_right _ _) h
   
-  def looseBvarUB_ir_lt_left
-    (h : (ir l r).looseBvarUB d < x)
+  def freeVarUB_ir_lt_left
+    (h : (ir l r).freeVarUB d < x)
   :
-    l.looseBvarUB d < x
+    l.freeVarUB d < x
   :=
     Nat.lt_of_le_of_lt (Nat.le_max_left _ _) h
   
-  def looseBvarUB_ir_lt_rite
-    (h : (ir l r).looseBvarUB d < x)
+  def freeVarUB_ir_lt_rite
+    (h : (ir l r).freeVarUB d < x)
   :
-    r.looseBvarUB d < x
+    r.freeVarUB d < x
   :=
     Nat.lt_of_le_of_lt (Nat.le_max_right _ _) h
   
-  def looseBvarUB_pair_le_left
-    (h : (pair l r).looseBvarUB d ≤ x)
+  def freeVarUB_pair_le_left
+    (h : (pair l r).freeVarUB d ≤ x)
   :
-    l.looseBvarUB d ≤ x
+    l.freeVarUB d ≤ x
   :=
     Nat.le_trans (Nat.le_max_left _ _) h
   
-  def looseBvarUB_pair_le_rite
-    (h : (pair l r).looseBvarUB d ≤ x)
+  def freeVarUB_pair_le_rite
+    (h : (pair l r).freeVarUB d ≤ x)
   :
-    r.looseBvarUB d ≤ x
+    r.freeVarUB d ≤ x
   :=
     Nat.le_trans (Nat.le_max_right _ _) h
   
-  def looseBvarUB_un_le_left
-    (h : (un l r).looseBvarUB d ≤ x)
+  def freeVarUB_un_le_left
+    (h : (un l r).freeVarUB d ≤ x)
   :
-    l.looseBvarUB d ≤ x
+    l.freeVarUB d ≤ x
   :=
     Nat.le_trans (Nat.le_max_left _ _) h
   
-  def looseBvarUB_un_le_rite
-    (h : (un l r).looseBvarUB d ≤ x)
+  def freeVarUB_un_le_rite
+    (h : (un l r).freeVarUB d ≤ x)
   :
-    r.looseBvarUB d ≤ x
+    r.freeVarUB d ≤ x
   :=
     Nat.le_trans (Nat.le_max_right _ _) h
   
-  def looseBvarUB_ir_le_left
-    (h : (ir l r).looseBvarUB d ≤ x)
+  def freeVarUB_ir_le_left
+    (h : (ir l r).freeVarUB d ≤ x)
   :
-    l.looseBvarUB d ≤ x
+    l.freeVarUB d ≤ x
   :=
     Nat.le_trans (Nat.le_max_left _ _) h
   
-  def looseBvarUB_ir_le_rite
-    (h : (ir l r).looseBvarUB d ≤ x)
+  def freeVarUB_ir_le_rite
+    (h : (ir l r).freeVarUB d ≤ x)
   :
-    r.looseBvarUB d ≤ x
+    r.freeVarUB d ≤ x
   :=
     Nat.le_trans (Nat.le_max_right _ _) h
   
   
-  def clearBvars_eq_of_ub
+  def clearVars_eq_of_ub
     {expr: Expr E}
     {ub: Nat}
-    (h: expr.looseBvarUB ≤ ub)
+    (h: expr.freeVarUB ≤ ub)
   :
-    Expr.clearBvars ub expr = expr
+    Expr.clearVars ub expr = expr
   :=
     let leL {l r} (h: max l r ≤ ub) := Nat.le_trans (Nat.le_max_left l r) h
     let leR {l r} (h: max l r ≤ ub) := Nat.le_trans (Nat.le_max_right l r) h
     match expr with
-    | .var _ _ => rfl
-    | .bvar _ => clearBvars_eq_bvar (Nat.lt_of_succ_le h)
+    | .const _ _ => rfl
+    | .var _ => clearVars_eq_var (Nat.lt_of_succ_le h)
     | .null => rfl
     | .pair _ _ =>
       congrArg₂ Expr.pair
-        (clearBvars_eq_of_ub (leL h))
-        (clearBvars_eq_of_ub (leR h))
+        (clearVars_eq_of_ub (leL h))
+        (clearVars_eq_of_ub (leR h))
     | .ir _ _ =>
       congrArg₂ Expr.ir
-        (clearBvars_eq_of_ub (leL h))
-        (clearBvars_eq_of_ub (leR h))
+        (clearVars_eq_of_ub (leL h))
+        (clearVars_eq_of_ub (leR h))
     | .condFull _ =>
-      congrArg Expr.condFull (clearBvars_eq_of_ub h)
+      congrArg Expr.condFull (clearVars_eq_of_ub h)
     | .compl _ =>
-      congrArg Expr.compl (clearBvars_eq_of_ub h)
+      congrArg Expr.compl (clearVars_eq_of_ub h)
     | .arbIr _ =>
       congrArg
         Expr.arbIr
-        (clearBvars_eq_of_ub (Nat.le_trans h (Nat.le_succ _)))
+        (clearVars_eq_of_ub (Nat.le_trans h (Nat.le_succ _)))
 end Expr
 
 namespace SingleLaneExpr
@@ -421,13 +421,13 @@ namespace SingleLaneExpr
     (dl: DefList)
     {expr: SingleLaneExpr}
     {bv: List Pair}
-    (h: expr.looseBvarUB ≤ bv.length)
+    (h: expr.freeVarUB ≤ bv.length)
     (rest: List Pair)
     (p: Pair)
   :
     expr.intp bv dl.wfm p ↔ expr.intp (bv ++ rest) dl.wfm p
   := by
     unfold SingleLaneExpr.intp
-    rw [SingleLaneExpr.clearBvars_preserves_interp_bv]
-    rw [Expr.clearBvars_eq_of_ub h]
+    rw [SingleLaneExpr.clearVars_preserves_interp_bv]
+    rw [Expr.clearVars_eq_of_ub h]
 end SingleLaneExpr
