Etst/WFC/Utils/Cause.lean
@@ -47,7 +47,7 @@ instance (D: Type*): HasSubset (Cause D) := ⟨Cause.IsSubset⟩
 -/
 inductive Cause.IsInapplicable
   (cause: Cause D)
-  (outSet: Set (ValVar D))
+  (outSet: Set (ValConst D))
   (b: Valuation D)
 :
   Prop
@@ -107,7 +107,7 @@ def Cause.IsWeaklySatisfiedBy.Not.toIsInapplicable
 def Cause.IsWeaklySatisfiedBy.toIsApplicable
   {b c: Valuation D}
   (isSat: Cause.IsWeaklySatisfiedBy cause b c)
-  (outSet: Set (ValVar D))
+  (outSet: Set (ValConst D))
   (outSetIsEmpty: ∀ {d x}, ⟨d, x⟩ ∈ outSet → ¬ (c x).posMem d)
 :
   ¬ Cause.IsInapplicable cause outSet b
